Improve documentation.

C1_Schreier_vector.v
@@ -1,6 +1,6 @@
 (* A functional Schreier-vector to compute orbits. *)
 
-From CGT Require Import A1_setup B1_fmap B2_perm B3_word B4_group.
+From CGT Require Import A1_setup A2_lists B1_fmap B2_perm B3_word B4_group.
 
 Module Schreier.
 Section Vector.
@@ -10,42 +10,42 @@ Definition vector := fmap perm.
 (* Add all numbers reachable from i. *)
 Fixpoint extend (i : positive) (h : perm)
   (gen : list perm) (V : vector)
-  (acc : list positive) :=
+  (dst : list positive) :=
   match gen with
-  | [] => (V, acc)
+  | [] => (V, dst)
   | g :: gen' =>
     let j := g⋅i in
     match lookup V j with
-    | Some _ => extend i h gen' V acc
-    | None => extend i h gen' (insert V j (g ∘ h)) (j :: acc)
+    | Some _ => extend i h gen' V dst
+    | None => extend i h gen' (insert V j (g ∘ h)) (j :: dst)
     end
   end.
 
 (* The generating set. *)
 Variable gen : list perm.
 
-(* Extend all numbers in the try list. *)
-Fixpoint extend_loop (V : vector) (try acc : list positive) :=
-  match try with
-  | [] => (V, acc)
-  | i :: try' =>
+(* Extend all numbers in the source list. *)
+Fixpoint extend_loop (V : vector) (src dst : list positive) :=
+  match src with
+  | [] => (V, dst)
+  | i :: src' =>
     match lookup V i with
-    | None => extend_loop V try' acc
+    | None => extend_loop V src' dst
     | Some h =>
-      match extend i h gen V acc with
-      | (V', acc') => extend_loop V' try' acc'
+      match extend i h gen V dst with
+      | (V', dst') => extend_loop V' src' dst'
       end
     end
   end.
 
 (* Repeat orbit extension n times. *)
-Fixpoint loop (V : vector) (try : list positive) (n : nat) :=
+Fixpoint loop (V : vector) (src : list positive) (n : nat) :=
   match n with
   | O => V
   | S m =>
-    match extend_loop V try [] with
+    match extend_loop V src [] with
     | (V', []) => V'
-    | (V', try') => loop V' try' m
+    | (V', src') => loop V' src' m
     end
   end.
 
@@ -78,11 +78,11 @@ Definition Sound (V : vector) := ∀i,
   | None => True
   end.
 
-Lemma sound_extend h gen' V acc :
+Lemma sound_extend h gen' V dst :
   Generates gen h -> gen' ⊆ gen ->
-  Sound V -> Sound (fst (extend h⋅k h gen' V acc)).
+  Sound V -> Sound (fst (extend h⋅k h gen' V dst)).
 Proof.
-revert V acc; simple_ind gen'.
+revert V dst; simple_ind gen'.
 apply incl_cons_inv in H0 as [].
 destruct (lookup _); apply IHgen'; try easy.
 intros j; rewrite lookup_insert.
@@ -90,23 +90,23 @@ destruct (_ =? _) eqn:E; [convert_bool; subst; split|apply H1].
 apply compose_generator; easy. apply apply_compose.
 Qed.
 
-Lemma sound_extend_loop V try acc :
-  Sound V -> Sound (fst (extend_loop V try acc)).
+Lemma sound_extend_loop V src dst :
+  Sound V -> Sound (fst (extend_loop V src dst)).
 Proof.
-revert V acc; simple_ind try.
-destruct (lookup V a) eqn:E. destruct (extend _) as [V' acc'] eqn:E'.
-replace V' with (fst (extend a p gen V acc)) by (rewrite E'; easy).
-all: apply IHtry. assert(Ha := H a); rewrite E in Ha; destruct Ha; subst.
+revert V dst; simple_ind src.
+destruct (lookup V a) eqn:E. destruct (extend _) as [V' dst'] eqn:E'.
+replace V' with (fst (extend a p gen V dst)) by (rewrite E'; easy).
+all: apply IHsrc. assert(Ha := H a); rewrite E in Ha; destruct Ha; subst.
 apply sound_extend; easy. easy.
 Qed.
 
-Lemma sound_loop V try n :
-  Sound V -> Sound (loop V try n).
+Lemma sound_loop V src n :
+  Sound V -> Sound (loop V src n).
 Proof.
-revert V try; simple_ind n.
-destruct (extend_loop _) as [V' try'] eqn:E.
-replace V' with (fst (extend_loop V try [])) by (rewrite E; easy).
-destruct try'. apply sound_extend_loop, H.
+revert V src; simple_ind n.
+destruct (extend_loop _) as [V' src'] eqn:E.
+replace V' with (fst (extend_loop V src [])) by (rewrite E; easy).
+destruct src'. apply sound_extend_loop, H.
 apply IHn, sound_extend_loop, H.
 Qed.
 
@@ -128,38 +128,29 @@ Local Open Scope nat.
 (* The vector contains the full orbit. *)
 Definition Complete (V : vector) := ∀π, Generates gen π -> Contains V π⋅k.
 
-Lemma complete_extend_loop_keep V try acc i :
-  Contains V i -> Contains (fst (extend_loop V try acc)) i.
+Lemma complete_extend_loop_keep V src dst i :
+  Contains V i -> Contains (fst (extend_loop V src dst)) i.
 Proof.
 Admitted.
 
-Lemma complete_loop_keep V try n i :
-  Contains V i -> Contains (loop V try n) i.
+Lemma complete_loop_keep V src n i :
+  Contains V i -> Contains (loop V src n) i.
 Proof.
 Admitted.
 
-Lemma complete_extend_loop_add V try acc V' try' σ i:
-  In σ gen -> In i try ->
-  extend_loop V try acc = (V', try') ->
-  ¬Contains V σ⋅i -> Contains V' σ⋅i /\ In σ⋅i try'.
+Lemma complete_extend_loop_add V src dst V' dst' σ i:
+  In σ gen -> In i src ->
+  extend_loop V src dst = (V', dst') ->
+  ¬Contains V σ⋅i -> Contains V' σ⋅i /\ In σ⋅i dst'.
 Proof.
 Admitted.
 
-Lemma complete_loop V try n i w :
-  w ⊆ gen -> length w <= n -> In i try ->
-  Contains V i -> Contains (loop V try n) (apply' w i).
+Lemma complete_loop V src i w :
+  w ⊆ gen -> In i src -> Contains V i ->
+  Contains (loop V src (length w)) (apply' w i).
 Proof.
-revert V try i w; induction n; simpl; intros.
-destruct w; easy. destruct (extend_loop _) as [V' try'] eqn:E.
-destruct w as [|σ w]; simpl.
-- (* The orbit point is already found. *)
-  assert(Contains V' i).
-  replace V' with (fst (extend_loop V try [])).
-  apply complete_extend_loop_keep, H2. rewrite E; easy.
-  destruct try'. apply H3. apply complete_loop_keep, H3.
-- (* We can apply an induction step. *)
-  (* Problem: what if σ⋅i is already contained in V? *)
-  (* Do we have to search w for a continuation point? *)
+apply rev_ind with (l:=w); clear w; [intros|intros σ w; intros]; simpl. easy.
+apply incl_app_inv in H0 as []; apply H in H2; try easy; clear H0 H1.
 Admitted.
 
 Theorem complete_build n :
@@ -167,7 +158,7 @@ Theorem complete_build n :
 Proof.
 intros H π [w []]; unfold build.
 destruct (short_connecting_word w k) as [w' [? []]].
-rewrite H1, apply_compose', <-H4. apply complete_loop.
+rewrite H1, apply_compose', <-H4.
 Admitted.
 
 End Completeness.
